some more work

theories/Metatheory.v
@@ -1,8 +1,11 @@
+From Coq Require Import Lia List FunctionalExtensionality.
 From Epic Require Export Syntax.
 From Epic Require Import FinUtil.
-From Coq Require Import Lia.
+
 
 Import ScopedNotations.
+Import ListNotations.
+
 
 Definition r_ctxt n := fin n -> nat.
 Definition e_ctxt m := fin m -> nat.
@@ -15,11 +18,52 @@ Definition sum {n} (c : fin n -> nat) (d : fin n -> nat) : fin n -> nat :=
 
 Definition zero {n} (x:fin n) : nat := 0.
 
-Definition one {n} (x:fin n) : fin n -> nat :=
-  fun (y : fin n) =>
-    if fin_eqb x y then 1 else 0.
+Lemma sum_zero_l : forall {n} (c : fin n -> nat),
+    sum c zero = c.
+Proof.
+  intros. apply functional_extensionality.
+  intros. unfold sum. unfold zero. lia.
+Qed.
 
-Definition SUM {n} (l : list (fin n -> nat)) : fin n -> nat :=
+Lemma sum_zero_r : forall {n} (c : fin n -> nat),
+    sum zero c = c.
+Proof.
+  intros. apply functional_extensionality.
+  intros. unfold sum. unfold zero. reflexivity.
+Qed.
+
+Definition delta {n} (x:fin n) (c:nat) : fin n -> nat :=
+  fun (y : fin n) =>
+    if fin_eqb x y then c else 0.
+
+Lemma delta_eq : forall n c (i1 i2 : fin n),
+    c <> 0 ->
+    delta i1 c i2 = c <-> i1 = i2.
+Proof.
+  intros.
+  unfold delta.
+  destruct (fin_eqb i1 i2) eqn:EQ.
+  rewrite fin_eqb_eq in EQ.
+  subst. tauto.
+  rewrite fin_eqb_neq in EQ.
+  split. intros; subst. contradiction. intros; contradiction.
+Qed.
+
+Lemma delta_neq : forall n c (i1 i2 : fin n),
+    delta i1 c i2 = 0  <-> (c = 0 \/ i1 <> i2).
+Proof.
+    intros. split; intros.
+    - destruct c. left; auto.
+      right. intros Heq. eapply delta_eq with (c:=S c) in Heq.
+      rewrite  H in Heq. discriminate.
+      intros C.  discriminate.
+    - destruct H.
+      + unfold delta. destruct (fin_eqb i1 i2) eqn: He; auto.
+      + unfold delta. destruct (fin_eqb i1 i2) eqn: He; auto. rewrite fin_eqb_eq in He.        contradiction.
+Qed.
+
+
+  Definition SUM {n} (l : list (fin n -> nat)) : fin n -> nat :=
   List.fold_right sum zero l.
 
 (*
@@ -48,7 +92,7 @@ Fixpoint ctxt_app' {n m : nat} (c : fin n -> nat) (d : fin m -> nat) :  fin (plu
 
 Definition ctxt_app {n m : nat} (c : fin n -> nat) (d : fin m -> nat) :  fin (plus n m) -> nat := scons_p n c d.
 
-Infix "⊎" := ctxt_app (at level 50).
+Infix "⊗" := ctxt_app (at level 50).
 
 Definition coerce {X} {n m} (c : fin (n + S m) -> X) : fin (S (n + m)) -> X.
   replace (n + S m) with (S (n + m)) in c by lia.
@@ -80,7 +124,7 @@ with wf_r_scope : forall (n m : nat), e_ctxt m -> r_ctxt n -> r_scope n m -> Pro
       (Δ' : r_ctxt n')
       (HΔ' : forall (r' : fin n'), Δ' r' = 2)
       (es : e_scope (n' + n) m)
-      (WFes : wf_e_scope (n' + n) m Γ (Δ' ⊎ Δ) es),
+      (WFes : wf_e_scope (n' + n) m Γ (Δ' ⊗ Δ) es),
       wf_r_scope n m Γ Δ (rbnd n' es)
 
 with wf_e_scope : forall (n m : nat), e_ctxt m -> r_ctxt n -> e_scope n m -> Prop :=
@@ -93,12 +137,12 @@ with wf_e_scope : forall (n m : nat), e_ctxt m -> r_ctxt n -> e_scope n m -> Pro
       (HΓ' : forall (e' : fin m'), Γ' e' = 1)      
       (stmts : list (stmt n (m' + m)))
       (GDs : list (e_ctxt (m' + m) * r_ctxt n))
-      (GS : (Γ' ⊎ Γ) = SUM (List.map fst GDs))
+      (GS : (Γ' ⊗ Γ) = SUM (List.map fst GDs))
       (DS : Δ = SUM (List.map snd GDs))
-      
       (WFstmts : List.Forall2
                    (fun s gd => wf_stmt n (m' + m) (fst gd) (snd gd) s) stmts GDs),
         wf_e_scope n m Γ Δ (ebnd m' stmts)
+
 with wf_stmt : forall (n m : nat), e_ctxt m -> r_ctxt n -> stmt n m -> Prop :=
 | wf_cut :
     forall n m
@@ -149,9 +193,85 @@ with wf_stmt : forall (n m : nat), e_ctxt m -> r_ctxt n -> stmt n m -> Prop :=
       (Δ : r_ctxt n)
       (HΔ : Δ = (one r)),
       wf_stmt n m Γ Δ (app (var_exp e) (var_res r)).
-  
-              
-              
+
+(*
+[λr0.
+  r0 = (r1, r1)]
+
+*)
+
+Example tm_id : tm 0 0 :=
+  lam (rbnd 1 (ebnd 0
+                 ([tup (var_res (var_zero))
+                     (List.map var_res ([shift (var_zero); shift (var_zero)])%list)]%list))).
+
+Lemma wf_tm_id : wf_tm 0 0 null tm_id.
+Proof.
+  econstructor.
+  - intros; auto. inversion e.
+  - eapply wf_rs with (Δ' := 2 .: null).
+    intros. inversion e.
+    auto_case. inversion f.
+    auto_case. inversion f.
+    eapply wf_es with (Γ' := zero).
+    intros. inversion e.
+    intros. inversion e'.
+    3 : { eapply Forall2_cons with (y := (null, _)).
+          eapply wf_tup with (Γ := null).
+          intros. inversion e.
+          simpl.  reflexivity.
+          eapply Forall2_nil. }
+    simpl. unfold ctxt_app. fsimpl. unfold sum.
+    apply functional_extensionality. intros. inversion x.
+    simpl. 
+    unfold ctxt_app.
+    fsimpl.
+    repeat rewrite sum_zero_l.
+    apply functional_extensionality. intros.
+    unfold one.
+    destruct (fin_eqb var_zero x) eqn:Hx.
+    rewrite fin_eqb_eq in Hx.
+    subst. fsimpl. 
+          
+          
+                
+    
+
+
+
+
+(* A "scope" picks out a list of statements from within a term *)
+Inductive scope (n m : nat) :=
+| here (n' m' : nat)   (* lam n' m'. [] *)
+| deeper (n' m' : nat) (i:nat) (rest : scope (n' + S n) (m' + m)).
+
+
+Inductive lookup_stmts : forall (n : nat) (m:nat) n' m' , tm n m -> scope n m -> list (stmt n' m') -> Prop :=
+| lookup_here : forall n m n' m' body,
+    lookup_stmts n m (n' + S n) (m' + m) (lam (rbnd n' (ebnd m' body))) (here n m n' m') body
+
+| lookup_deeper : forall n m n' m' n'' m'' i (rest : scope _ _ ) body body1 r t body2,
+    length body1 = i ->
+    lookup_stmts (n' + S n) (m' + m) n'' m'' t rest body ->
+    
+    lookup_stmts n m n'' m''
+      (lam (rbnd n' (ebnd m' (body1 ++ [def r t] ++ body2)))) (deeper _ _ n' m' i rest) body.
+
+
+
+
+Inductive tm_redex (n m : nat) :=
+| lam_r (n' m' : nat) (s : body_redex (n' + S n) (m' + m))
+with body_redex (n m : nat) :=
+| cut_r (i:nat) (r1 r2 : fin n)
+| tup_r (i j:nat) (H:i<>j) (r1 : fin n) (rs rs' : list (fin n))
+| app_local_r (i j k :nat) (H1:i<>j) (H2:j<>k) (H3:i<>k) (re : fin n) (t: tm n m) (e : fin m) (r : fin n)
+| app_deep_r (i j k : nat) 
+
+Scheme mut_tm_path := Induction for tm_path Sort Prop
+with mut_stmts_path := Induction for stmts_path Sort Prop.
+
+
 
 
 (*
